src/lowparse/LowParse.Low.VLGen.fst
@@ -1,13 +1,14 @@
 module LowParse.Low.VLGen
 include LowParse.Spec.VLGen
 include LowParse.Low.VLData
+include LowParse.Low.BoundedInt // for jump_bounded_int32
 
 module U32 = FStar.UInt32
 module HST = FStar.HyperStack.ST
 
 #reset-options "--z3cliopt smt.arith.nl=false"
 
-#push-options "--z3rlimit 16 --max_ifuel 8"
+#push-options "--z3rlimit 32 --max_ifuel 8"
 
 inline_for_extraction
 let validate_bounded_vlgen
@@ -42,6 +43,43 @@ let validate_bounded_vlgen
     validate_fldata_strong s v (U32.v len) len input n
 
 inline_for_extraction
+let validate_bounded_vlgen'
+  (vmin: der_length_t)
+  (min: U32.t { U32.v min == vmin } )
+  (vmax: der_length_t)
+  (max: U32.t { U32.v max == vmax /\ U32.v min <= U32.v max } )
+  (#sk: parser_kind)
+  (#pk: parser sk U32.t)
+  (vk: validator pk)
+  (rk: leaf_reader pk)
+  (#k: parser_kind)
+  (#t: Type)
+  (#p: parser k t)
+  (s: serializer p)
+  (v: validator p)
+: Tot (validator (parse_bounded_vlgen' (vmin) (vmax) pk s))
+= fun #rrel #rel input pos ->
+  let h = HST.get () in
+  [@inline_let] let _ =
+    valid_facts (parse_bounded_vlgen' (U32.v min) (U32.v max) pk s) h input pos;
+    parse_bounded_vlgen_unfold (U32.v min) (U32.v max) (parse_bounded_int32 vmin vmax pk) s (bytes_of_slice_from h input pos);
+    parse_bounded_int32_unfold vmin vmax pk (bytes_of_slice_from h input pos);
+    valid_facts pk h input pos
+  in
+  let n = vk input pos in
+  if validator_max_length `U32.lt` n
+  then n
+  else
+    let len = rk input pos in
+    if len `U32.lt` min || max `U32.lt` len
+    then
+      validator_error_generic
+    else
+      [@inline_let]
+      let _ = valid_facts (parse_fldata_strong s (U32.v len)) h input n in
+      validate_fldata_strong s v (U32.v len) len input n
+
+inline_for_extraction
 let validate_vlgen
   (vmin: der_length_t)
   (min: U32.t { U32.v min == vmin } )
@@ -59,6 +97,27 @@ let validate_vlgen
 : Tot (validator (parse_vlgen (vmin) (vmax) pk s))
 = validate_synth
     (validate_bounded_vlgen vmin min vmax max vk rk s v)
+    (synth_vlgen (U32.v min) (U32.v max) s)
+    ()
+
+inline_for_extraction
+let validate_vlgen'
+  (vmin: der_length_t)
+  (min: U32.t { U32.v min == vmin } )
+  (vmax: der_length_t)
+  (max: U32.t { U32.v max == vmax /\ U32.v min <= U32.v max } )
+  (#sk: parser_kind)
+  (#pk: parser sk U32.t)
+  (vk: validator pk)
+  (rk: leaf_reader pk)
+  (#k: parser_kind)
+  (#t: Type)
+  (#p: parser k t)
+  (s: serializer p { parse_vlgen_precond (U32.v min) (U32.v max) k })
+  (v: validator p)
+: Tot (validator (parse_vlgen' (vmin) (vmax) pk s))
+= validate_synth
+    (validate_bounded_vlgen' vmin min vmax max vk rk s v)
     (synth_vlgen (U32.v min) (U32.v max) s)
     ()
 
@@ -90,6 +149,22 @@ let jump_bounded_vlgen
   jump_fldata_strong s (U32.v len) len input n
 
 inline_for_extraction
+let jump_bounded_vlgen'
+  (vmin: der_length_t)
+  (vmax: der_length_t { vmin <= vmax /\ vmax < 4294967296 } )
+  (#sk: parser_kind)
+  (#pk: parser sk U32.t)
+  (vk: jumper pk)
+  (rk: leaf_reader pk)
+  (#k: parser_kind)
+  (#t: Type)
+  (#p: parser k t)
+  (s: serializer p)
+  (v: jumper p)
+: Tot (jumper (parse_bounded_vlgen' (vmin) (vmax) pk s))
+= jump_bounded_vlgen vmin vmax (jump_bounded_int32 (U32.uint_to_t vmin) (U32.uint_to_t vmax) vk) (read_bounded_int32 (U32.uint_to_t vmin) (U32.uint_to_t vmax) rk) s v
+
+inline_for_extraction
 let jump_vlgen
   (vmin: der_length_t)
   (vmax: der_length_t { vmin <= vmax /\ vmax < 4294967296 } )
@@ -107,6 +182,22 @@ let jump_vlgen
     (jump_bounded_vlgen vmin vmax vk rk s v)
     (synth_vlgen (vmin) (vmax) s)
     ()
+
+inline_for_extraction
+let jump_vlgen'
+  (vmin: der_length_t)
+  (vmax: der_length_t { vmin <= vmax /\ vmax < 4294967296 } )
+  (#sk: parser_kind)
+  (#pk: parser sk U32.t)
+  (vk: jumper pk)
+  (rk: leaf_reader pk)
+  (#k: parser_kind)
+  (#t: Type)
+  (#p: parser k t)
+  (s: serializer p { parse_vlgen_precond (vmin) (vmax) k })
+  (v: jumper p)
+: Tot (jumper (parse_vlgen' (vmin) (vmax) pk s))
+= jump_vlgen vmin vmax (jump_bounded_int32 (U32.uint_to_t vmin) (U32.uint_to_t vmax) vk) (read_bounded_int32 (U32.uint_to_t vmin) (U32.uint_to_t vmax) rk) s v
 
 let gaccessor_bounded_vlgen_payload
   (min: nat)
@@ -127,6 +218,18 @@ let gaccessor_bounded_vlgen_payload
       (sz, Seq.length input - sz)
   in
   (res <: (res : _ { gaccessor_post' (parse_bounded_vlgen min max pk s) p (clens_bounded_vldata_strong_payload min max s) input res } ))
+
+let gaccessor_bounded_vlgen'_payload
+  (min: nat)
+  (max: nat { min <= max /\ max > 0 /\ max < 4294967296 } )
+  (#sk: parser_kind)
+  (pk: parser sk U32.t)
+  (#k: parser_kind)
+  (#t: Type0)
+  (#p: parser k t)
+  (s: serializer p)
+: Tot (gaccessor (parse_bounded_vlgen' min max pk s) p (clens_bounded_vldata_strong_payload min max s))
+= gaccessor_bounded_vlgen_payload min max (parse_bounded_int32 min max pk) s
 
 module B = LowStar.Buffer
 
@@ -154,6 +257,20 @@ let accessor_bounded_vlgen_payload
   in
   jk input pos
 
+inline_for_extraction
+let accessor_bounded_vlgen'_payload
+  (min: nat)
+  (max: nat { min <= max /\ max > 0 /\ max < 4294967296 } )
+  (#sk: parser_kind)
+  (#pk: parser sk U32.t)
+  (jk: jumper pk)
+  (#k: parser_kind)
+  (#t: Type0)
+  (#p: parser k t)
+  (s: serializer p)
+: Tot (accessor (gaccessor_bounded_vlgen'_payload min max pk s))
+= accessor_bounded_vlgen_payload min max (jump_bounded_int32 (U32.uint_to_t min) (U32.uint_to_t max) jk) s
+
 let gaccessor_vlgen_payload
   (min: nat)
   (max: nat { min <= max /\ max > 0 /\ max < 4294967296 } )
@@ -173,6 +290,18 @@ let gaccessor_vlgen_payload
       (sz, Seq.length input - sz)
   in
   (res <: (res : _ { gaccessor_post' (parse_vlgen min max pk s) p (clens_id _) input res } ))
+
+let gaccessor_vlgen'_payload
+  (min: nat)
+  (max: nat { min <= max /\ max > 0 /\ max < 4294967296 } )
+  (#sk: parser_kind)
+  (pk: parser sk U32.t)
+  (#k: parser_kind)
+  (#t: Type0)
+  (#p: parser k t)
+  (s: serializer p { parse_vlgen_precond min max k } )
+: Tot (gaccessor (parse_vlgen' min max pk s) p (clens_id _))
+= gaccessor_vlgen_payload min max (parse_bounded_int32 min max pk) s
 
 inline_for_extraction
 let accessor_vlgen_payload
@@ -197,6 +326,20 @@ let accessor_vlgen_payload
     parse_strong_prefix pk (bytes_of_slice_from h input pos) (bytes_of_slice_from_to h input pos (pos `U32.add` U32.uint_to_t (content_length (parse_vlgen min max pk s) h input pos)))
   in
   jk input pos
+
+inline_for_extraction
+let accessor_vlgen'_payload
+  (min: nat)
+  (max: nat { min <= max /\ max > 0 /\ max < 4294967296 } )
+  (#sk: parser_kind)
+  (#pk: parser sk U32.t)
+  (jk: jumper pk { sk.parser_kind_subkind == Some ParserStrong } )
+  (#k: parser_kind)
+  (#t: Type0)
+  (#p: parser k t)
+  (s: serializer p { parse_vlgen_precond min max k } )
+: Tot (accessor (gaccessor_vlgen'_payload min max pk s))
+= accessor_vlgen_payload min max (jump_bounded_int32 (U32.uint_to_t min) (U32.uint_to_t max) jk) s
 
 module HS = FStar.HyperStack
 
